\section{Allgemeines}

\begin{equation*}
    x(t) = \sum_{k=-\infty}^{\infty} \delta(t - kT_s) \knochen \sum_{k=-\infty}^{\infty} e^{-j2\pi fkT_s}
\end{equation*}

\subsection{Impulseantwort}

\begin{equation*}
    \delta[k] = \begin{cases}
        1 & \hspace{5mm} k=0 \\
        0 & \hspace{5mm} k \neq 0 \\
    \end{cases}
\end{equation*}

\subsection{Diskrete Faltung}

\begin{equation*}
    y[k] = x[.] \star h[.] = \sum_{i=-\infty}^{\infty} x[i]\cdot h[k-i] = \sum_{i=-\infty}^{\infty} x[k-i] \cdot h[i]
\end{equation*}

\subsection{Normierte (Kreis-) Frequenz}

\begin{align*}
    f_n    &= f T_s = \frac{f}{f_s}                     &\hspace{8mm}\textrm{Normierte Frequenz} \\
    \Omega &= 2\pi f_n = 2\pi f T_s = 2\pi\frac{f}{f_s} &\hspace{8mm}\textrm{Normierte Kreisfrequenz} \\
\end{align*}

\subsection{Komplexer Frequenzgang}
\begin{align*}
    \underline{H}(\Omega) &= \sum_{m=-\infty}^{\infty} h[m] e^{-j\Omega \cdot m} \\
    \underline{H}(f)      &= \sum_{m=-\infty}^{\infty} h[m] e^{-j2\pi f m T}
\end{align*}


